more work on poly method

Code/Examples/Map.v
@@ -1,4 +1,5 @@
-Require Import Prelude.CompatibleRelation.
+Require Import Lia.
+Require Import Prelude.Orders.
 Require Import Syntax.Signature.
 Require Import Syntax.StrongNormalization.SN.
 Require Import Interpretation.WeaklyMonotonicAlgebra.
@@ -8,15 +9,13 @@ Require Import Interpretation.OrderInterpretation.
 Local Open Scope nat.
 
 Inductive base_types : Type :=
-| TNat   : base_types
+| TBtype : base_types
 | TList  : base_types.
 
-Definition Nat : ty base_types := Base TNat.
+Definition Btype : ty base_types := Base TBtype.
 Definition List : ty base_types := Base TList.
 
 Inductive fun_symbols : Type :=
-| TZero  : fun_symbols
-| TSucc  : fun_symbols
 | TNil   : fun_symbols
 | TCons  : fun_symbols
 | TMap   : fun_symbols.
@@ -25,22 +24,10 @@ Definition map_ar
            (f : fun_symbols)
   : ty base_types
   := match f with
-     | TZero  => Nat
-     | TSucc  => Nat ⟶ Nat
      | TNil   => List
-     | TCons  => Nat ⟶ List ⟶ List
-     | TMap   => (Nat ⟶ Nat) ⟶ List ⟶ List
+     | TCons  => Btype ⟶ List ⟶ List
+     | TMap   => (Btype ⟶ Btype) ⟶ List ⟶ List
      end.
-
-Definition Zero
-           {C : con base_types}
-  : tm map_ar C Nat
-  := BaseTm TZero.
-
-Definition Suc
-           {C : con base_types}
-  : tm map_ar C (Nat ⟶ Nat)
-  := BaseTm TSucc.
 
 Definition Nil
            {C : con base_types}
@@ -49,18 +36,18 @@ Definition Nil
 
 Definition Cons
            {C : con base_types}
-  : tm map_ar C (Nat ⟶ List ⟶ List)
+  : tm map_ar C (Btype ⟶ List ⟶ List)
   := BaseTm TCons.
 
 Definition Map
            {C : con base_types}
-  : tm map_ar C ((Nat ⟶ Nat) ⟶ List ⟶ List)
+  : tm map_ar C ((Btype ⟶ Btype) ⟶ List ⟶ List)
   := BaseTm TMap.
 
 Definition map_nil
   : rewriteRule map_ar
   := make_rewrite
-       ((Nat ⟶ Nat) ,, ∙)
+       ((Btype ⟶ Btype) ,, ∙)
        List
        (let f := TmVar Vz in
         Map · f · Nil)
@@ -69,7 +56,7 @@ Definition map_nil
 Definition map_cons
   : rewriteRule map_ar
   := make_rewrite
-       ((Nat ⟶ Nat) ,, Nat ,, List ,, ∙)
+       ((Btype ⟶ Btype) ,, Btype ,, List ,, ∙)
        List
        (let f := TmVar Vz in
         let x := TmVar (Vs Vz) in
@@ -92,95 +79,38 @@ Definition map_fun_poly
            (f : fun_symbols)
   : poly ∙ (arity map_afs f)
   := match f with
-     | TZero =>
-       P_base (P_const 1)
-     | TSucc =>
-       λP
-       let x := P_var Vz in
-       P_base (from_poly x +P P_const 1)
      | TNil =>
-       P_base (P_const 1)
+       P_base (P_const 2)
      | TCons =>
        λP
-       let x := P_var Vz in
+       let y0 := P_var Vz in
        λP
-       let xs := P_var (Vs Vz) in
-       P_base (P_const 1 +P (from_poly x +P from_poly xs))
+       let y1 := P_var (Vs Vz) in
+       P_base (P_const 3 +P from_poly y0 +P from_poly y1)
      | TMap =>
        λP
-       let xs := P_var Vz in
+       let y0 := P_var Vz in
        λP
-       let f := P_var (Vs Vz) in
-       P_base (P_const 1 +P ((P_const 1 +P from_poly xs) *P from_poly (f ·P P_base (from_poly xs))))
+       let G1 := P_var (Vs Vz) in
+       P_base (P_const 3
+              +P (P_const 3) *P (from_poly y0)
+              +P from_poly (G1 ·P P_base (from_poly y0))
+              +P (P_const 3) *P (from_poly y0) *P from_poly (G1 ·P P_base (from_poly y0)))
      end.
 
-Close Scope poly_scope.
-
-(*
-Notation "0" := (P_const 0).
-Notation "1" := (P_const 1).
-Notation "2" := (P_const 2).
-Notation "3" := (P_const 3).
-
-Definition map_fun_poly
-  : forall f : fun_symbols, poly ∙ (arity map_afs f)
-  := fun f =>
-     match f with
-     | TZero =>
-       P_base 1
-     | TSucc =>
-       λP
-       let x := P_var Vz in
-       P_base (from_poly x +P 1)
-     | TNil =>
-       P_base 1
-     | TCons =>
-       λP
-       let x := P_var Vz in
-       λP
-       let xs := P_var (Vs Vz) in
-       P_base (1 +P (from_poly x +P from_poly xs))
-     | TMap =>
-       λP
-       let xs := P_var Vz in
-       λP
-       let f := P_var (Vs Vz) in
-       P_base (1 +P ((1 +P from_poly xs) *P from_poly (f ·P P_base (from_poly xs))))
-     end.
- *)
-
-(*
 Definition map_isSN
   : isSN map_afs.
 Proof.
   apply afs_is_SN_from_Alg.
-  simple refine (poly_WMalgebra _ _ _ _ _ _ _).
+  simple refine (poly_WMalgebra _ _ _).
   - exact map_fun_poly.
-  - intros A1 A2.
-    refine (P_app _ _).
-    + apply P_var.
-      apply Vz.
-    + apply P_var.
-      apply Vs.
-      apply Vz.
-  - intros A1 A2 f x.
-    cbn.
-    apply ge_refl.
-  - intros A1 A2 f1 f2 x Hf.
-    cbn.
-    apply Hf.
-  - intros A1 A2 f x1 x2 Hx.
-    cbn.
-    admit.
   - intros r x.
-    cbn in *.
     destruct r as [ r Hr ].
-    repeat (destruct Hr as [ | Hr ]) ; try subst ; cbn in *.
-    + destruct x ; cbn in *.
+    repeat (destruct Hr as [ | Hr ]) ; try subst ; cbn -[Nat.add Nat.mul].
+    + nia.
+    + rewrite !PeanoNat.Nat.mul_0_l.
+      rewrite !plus_O_n.
+      rewrite <- !plus_n_O.
       admit.
-    + destruct x as [ f [ x1 [ x2 [ ] ] ] ].
-      nia.
-      admit.
-    + contradiction.
+    + destruct Hr.
 Admitted.
- *)
