Code/Interpretation/Polynomial.v
@@ -1,12 +1,14 @@
 Require Import Prelude.Funext.
 Require Import Prelude.WellfoundedRelation.
-Require Import Prelude.CompatibleRelation.
+Require Import Prelude.Orders.
 Require Import Prelude.Lexico.
 Require Import Syntax.Signature.
 Require Import Syntax.StrongNormalization.SN.
 Require Import Syntax.StrongNormalization.BetaReductionSN.
 Require Import Interpretation.OrderInterpretation.
 Require Import Interpretation.WeaklyMonotonicAlgebra.
+
+Require Import Lia.
 
 Declare Scope poly_scope.
 
@@ -66,63 +68,196 @@ with sem_poly
 Notation "⟦ P ⟧" := (sem_poly P).
 Notation "⟦ P ⟧B" := (sem_base_poly P).
 
-Definition prod_unit_map
-           (A B : CompatRel)
-  : weakMonotoneMap (A * B) (A * (B * unit_CompatRel)).
-Proof.
-  unshelve esplit.
-  - exact (fun z => (fst z , (snd z , tt))).
-  - intros z1 z2 p ; cbn.
-    repeat split ; auto.
-    + apply p.
-    + apply p.
-Defined.
-
 Section PolyAlgebra.
   Context {B : Type} {F : Type}
           (X : afs B F)
-          (P : forall (f : F), poly ∙ (arity X f))
-          (app : forall (A1 A2 : ty B), poly ((A1 ⟶ A2) ,, A1 ,, ∙) A2).
+          (P : forall (f : F), poly ∙ (arity X f)).
 
   Definition p_base : B -> CompatRel
-    := fun _ : B => nat_CompatRel.
+    := fun (_ : B) => nat_CompatRel.
 
   Definition p_tm (f : F) : sem_Ty p_base (arity X f)
     := sem_poly (P f) tt.
+  
+  Fixpoint minimal_element_sem_ty
+           (A : ty B)
+    : minimal_element (sem_Ty p_base A)
+    := match A with
+       | Base _ => nat_minimal_element
+       | A1 ⟶ A2 => min_el_fun_space _ (minimal_element_sem_ty A2)
+       end.
 
-  Definition p_app (A1 A2 : ty B)
-    := comp_WM
-         (prod_unit_map
-            (sem_Ty p_base (A1 ⟶ A2))
-            (sem_Ty p_base A1))
-         (sem_poly (app A1 A2)).
+  Fixpoint lower_value_function
+           (A : ty B)
+    : sem_Ty p_base A ⇒ nat_CompatRel
+    := match A with
+       | Base _ => id_WM nat_CompatRel
+       | A₁ ⟶ A₂ => apply_el_WM (lower_value_function A₂) (minimal_element_sem_ty A₁)
+       end.
+
+  Fixpoint plus_ty_nat
+           (A : ty B)
+    : sem_Ty p_base A * nat_CompatRel ⇒ sem_Ty p_base A
+    := match A with
+       | Base _ => plus_as_weakMonotoneMap
+       | A₁ ⟶ A₂ =>
+           lambda_abs
+             (comp_WM
+                (pair_WM
+                   (app_WM
+                      (comp_WM (snd_WM _ _) (fst_WM _ _))
+                      (fst_WM _ _))
+                   (comp_WM (snd_WM _ _) (snd_WM _ _)))
+                (plus_ty_nat A₂))
+       end.
+
+  Fixpoint plus_ty
+           (A : ty B)
+    : sem_Ty p_base A * sem_Ty p_base A ⇒ sem_Ty p_base A
+    := match A with
+       | Base _ => plus_as_weakMonotoneMap
+       | A₁ ⟶ A₂ =>
+           lambda_abs
+             (comp_WM
+                (pair_WM
+                   (app_WM
+                      (comp_WM (snd_WM _ _) (fst_WM _ _))
+                      (fst_WM _ _))
+                   (app_WM
+                      (comp_WM (snd_WM _ _) (snd_WM _ _))
+                      (fst_WM _ _)))
+                (plus_ty A₂))
+       end.
+             
+  Fixpoint sum_of_lower_value_function
+           (A : ty B)
+    : sem_Ty p_base A
+    := match A with
+       | Base _ => 0
+       | A₁ ⟶ A₂ =>
+           make_monotone
+             (fun x => plus_ty_nat
+                         A₂
+                         (sum_of_lower_value_function _
+                          ,
+                          lower_value_function _ x))
+             _
+       end.
+  
+  Definition p_app_fun
+             {A1 A2 : ty B}
+    : sem_Ty p_base (A1 ⟶ A2) * sem_Ty p_base A1 -> sem_Ty p_base A2
+    := fun z =>
+         let f := fst z in
+         let x := snd z in
+         plus_ty
+           _
+           (plus_ty_nat
+              _
+              (sum_of_lower_value_function _
+               ,
+               lower_value_function _ f + lower_value_function _ x)
+            ,
+            f x).
+
+  Global Instance weakMonotone_p_app_fun
+                  (A1 A2 : ty B)
+    : @weakMonotone
+        (sem_Ty p_base (A1 ⟶ A2) * sem_Ty p_base A1)
+        (sem_Ty p_base A2)
+        p_app_fun.
+  Proof.
+    intros x₁ x₂ p.
+    unfold p_app_fun.
+    apply map_ge.
+    split.
+    - cbn.
+      apply map_ge.
+      split.
+      * apply ge_refl.
+      * assert (lower_value_function A1 (snd x₁)
+                >=
+                lower_value_function A1 (snd x₂)).
+        {
+          apply map_ge.
+          apply p.
+        }
+        assert (lower_value_function A2 (fst x₁ (minimal_element_sem_ty A1))
+                >=
+                lower_value_function A2 (fst x₂ (minimal_element_sem_ty A1))).
+        {
+          apply map_ge.
+          apply p.
+        }
+        cbn in *.
+        nia.
+    - cbn.
+      cbn in p.
+      destruct p as [ p1 p2 ].
+      refine (ge_trans (p1 _) _).
+      apply map_ge.
+      apply p2.
+  Qed.
+  
+  Definition p_app
+             (A1 A2 : ty B)
+    : sem_Ty p_base (A1 ⟶ A2) * sem_Ty p_base A1 ⇒ sem_Ty p_base A2
+    := @make_monotone
+         (sem_Ty p_base (A1 ⟶ A2) * sem_Ty p_base A1)
+         (sem_Ty p_base A2)
+         p_app_fun
+         _.
+
+  Proposition p_app_ge_id
+              (A₁ A₂ : ty B)
+              (f : sem_Ty p_base A₁ ⇒ sem_Ty p_base A₂)
+              (x : sem_Ty p_base A₁)
+    : p_app_fun (f , x) >= f x.
+  Proof.
+  Admitted.
+
+  Proposition p_app_strict_l
+              (A₁ A₂ : ty B)
+              (f₁ f₂ : sem_Ty p_base A₁ ⇒ sem_Ty p_base A₂)
+              (x : sem_Ty p_base A₁)
+              (p : f₁ > f₂)
+    : p_app_fun (f₁ , x) > p_app_fun (f₂ , x).
+  Proof.
+  Admitted.
+
+  Proposition p_app_strict_r
+              (A₁ A₂ : ty B)
+              (f : sem_Ty p_base A₁ ⇒ sem_Ty p_base A₂)
+              (x₁ x₂ : sem_Ty p_base A₁)
+              (p : x₁ > x₂)
+    : p_app_fun (f , x₁) > p_app_fun (f , x₂).
+  Proof.
+  Admitted.
+
+  Definition poly_WMalgebra_rewrite_rules
+             (H : forall (r : rewriteRules X)
+                         (x : sem_Con p_base (vars r)),
+                  sem_Tm p_base p_tm p_app (lhs r) x
+                  >
+                  sem_Tm p_base p_tm p_app (rhs r) x)
+             (r : rewriteRules X)
+             (C : con B)
+             (s : sub (arity X) C (vars r))
+             (x : sem_Con p_base C)
+    : sem_Tm p_base p_tm p_app (subTm (lhs r) s) x
+      >
+      sem_Tm p_base p_tm p_app (subTm (rhs r) s) x.
+  Proof.
+    rewrite !sub_Lemma.
+    apply H.
+  Qed.
   
   Definition poly_WMalgebra
-             (H1 : forall (A1 A2 : ty B)
-                          (f : weakMonotoneMap (sem_Ty p_base A1) (sem_Ty p_base A2))
-                          (x : sem_Ty p_base A1),
-                 ⟦ app A1 A2 ⟧ (f , (x , tt)) >= f x)
-             (H2 : forall (A1 A2 : ty B)
-                          (f1 f2 : weakMonotoneMap (sem_Ty p_base A1) (sem_Ty p_base A2))
-                          (x : sem_Ty p_base A1),
-                 (forall z, f1 z > f2 z)
-                 ->
-                 ⟦ app A1 A2 ⟧ (f1, (x, tt))
-                 >
-                 ⟦ app A1 A2 ⟧ (f2 , (x , tt)))
-             (H3 : forall (A1 A2 : ty B)
-                          (f : weakMonotoneMap (sem_Ty p_base A1) (sem_Ty p_base A2))
-                          (x1 x2 : sem_Ty p_base A1),
-                 x1 > x2
-                 ->
-                 ⟦ app A1 A2 ⟧ (f , (x1 , tt))
-                 >
-                 ⟦ app A1 A2 ⟧ (f , (x2 , tt)))
-             (H4 : forall (r : rewriteRules X)
-                          (x : sem_Con p_base (vars r)),
-                 sem_Tm p_base p_tm p_app (lhs r) x
-                 >
-                 sem_Tm p_base p_tm p_app (rhs r) x)
+             (H : forall (r : rewriteRules X)
+                         (x : sem_Con p_base (vars r)),
+                  sem_Tm p_base p_tm p_app (lhs r) x
+                  >
+                    sem_Tm p_base p_tm p_app (rhs r) x)
     : WMalgebra X.
   Proof.
     simple refine (make_WMalgebra
@@ -133,216 +268,10 @@ Section PolyAlgebra.
                      _
                      p_tm
                      p_app
-                     H1 H2 H3 _).
-    - intros r C s x.
-      rewrite !sub_Lemma.
-      apply H4.
+                     _ _ _ _).
+    - exact p_app_ge_id.
+    - exact p_app_strict_l.
+    - exact p_app_strict_r.
+    - exact (poly_WMalgebra_rewrite_rules H).
   Defined.
 End PolyAlgebra.
-
-
-(*
-Inductive base_poly {B : Type} : con B -> Type :=
-| P_const : forall (C : con B), nat -> base_poly C
-| P_plus : forall (C : con B), base_poly C -> base_poly C -> base_poly C
-| P_mult : forall (C : con B), base_poly C -> base_poly C -> base_poly C
-| P_b_app : forall (C : con B) (A : ty B) (b : B),
-              poly C (A ⟶ Base b)
-              -> poly C A
-              -> base_poly C
-| P_b_var : forall (C : con B) (b : B), var C (Base b) -> base_poly C
-with poly {B : Type} : con B -> ty B -> Type :=
-| P_base : forall (C : con B) (b : B), base_poly C -> poly C (Base b)
-| P_var : forall (C : con B) (A : ty B),
-            var C A
-            -> poly C A
-| P_app : forall (C : con B) (A₁ A₂ : ty B),
-            poly C (A₁ ⟶ A₂)
-            -> poly C A₁
-            -> poly C A₂
-| P_lam : forall (C : con B) (A₁ A₂ : ty B),
-            poly (A₁ ,, C) A₂
-            -> poly C (A₁ ⟶ A₂).
-*)
-(*
-Inductive poly {B : Type} : con B -> ty B -> Type :=
-| P_const : forall (C : con B) (b : B),
-              nat -> poly C (Base b)
-| P_plus : forall (C : con B) (b₁ b₂ b₃ : B),
-              poly C (Base b₁)
-              -> poly C (Base b₂)
-              -> poly C (Base b₃)
-| P_mult : forall (C : con B) (b₁ b₂ b₃ : B),
-              poly C (Base b₁)
-              -> poly C (Base b₂)
-              -> poly C (Base b₃)
-| P_var : forall (C : con B) (A : ty B),
-            var C A
-            -> poly C A
-| P_app : forall (C : con B) (A₁ A₂ : ty B),
-            poly C (A₁ ⟶ A₂)
-            -> poly C A₁
-            -> poly C A₂
-| P_lam : forall (C : con B) (A₁ A₂ : ty B),
-            poly (A₁ ,, C) A₂
-            -> poly C (A₁ ⟶ A₂).
-
-
-Definition sem_poly
-         {B : Type}
-         {C : con B}
-         {A : ty B}
-         (P : poly C A)
-  : weakMonotoneMap
-      (sem_Con (fun _ => nat_CompatRel) C)
-      (sem_Ty (fun _ => nat_CompatRel) A).
-Proof.
-  induction P.
-  - apply (const_WM _ nat_CompatRel n).
-  - apply (plus_WM IHP1 IHP2).
-  - apply (mult_WM IHP1 IHP2).
-  - apply (sem_Var (fun _ => nat_CompatRel) v).
-  - apply (app_WM IHP1 IHP2).
-  - apply (lambda_abs IHP).
-Defined.
-
-(*
-Inductive poly {B : Type} : con B -> ty B -> Type :=
-| P_const   : forall (C : con B) (b : B),
-                nat -> poly C (Base b)
-| P_plus    : forall {C : con B} {b : B},
-                poly C (Base b)
-                -> poly C (Base b)
-                -> poly C (Base b)
-| P_mult    : forall {C : con B} {b : B},
-                poly C (Base b)
-                -> poly C (Base b)
-                -> poly C (Base b)
-| P_base    : forall {C : con B} {b : B},
-                base_poly C (Base b)
-                -> poly C (Base b)
-| P_lam     : forall {C : con B} {A1 A2 : ty B},
-                poly (A1 ,, C) A2
-                -> poly C (A1 ⟶ A2)
-with base_poly {B : Type} : con B -> ty B -> Type :=
-| PVar      : forall {C : con B} {A : ty B},
-                var C A
-                -> base_poly C A
-| Papp      : forall {C : con B} {A B : ty B},
-                base_poly C (A ⟶ B)
-                -> poly C A
-                -> base_poly C B.
-
-Fixpoint sem_poly
-         {B : Type}
-         {C : con B}
-         {A : ty B}
-         (P : poly C A)
-  : weakMonotoneMap
-      (sem_Con (fun _ => nat_CompatRel) C)
-      (sem_Ty (fun _ => nat_CompatRel) A)
-  := match P with
-     | P_const _ _ n  => const_WM _ nat_CompatRel n
-     | P_plus P1 P2   => plus_WM (sem_poly P1) (sem_poly P2)
-     | P_mult P1 P2   => mult_WM (sem_poly P1) (sem_poly P2)
-     | P_base P       => sem_base_poly P
-     | P_lam P        => lambda_abs (sem_poly P)
-     end
-with sem_base_poly
-     {B : Type}
-     {C : con B}
-     {A : ty B}
-     (P : base_poly C A)
-  : weakMonotoneMap
-      (sem_Con (fun _ => nat_CompatRel) C)
-      (sem_Ty (fun _ => nat_CompatRel) A)
-  := match P with
-     | PVar v         => sem_Var (fun _ => nat_CompatRel) v
-     | Papp P1 P2     => app_WM (sem_base_poly P1) (sem_poly P2)
-     end.
-
-Definition prod_unit_map
-           (A B : CompatRel)
-  : weakMonotoneMap (A * B) (A * (B * unit_CompatRel)).
-Proof.
-  unshelve esplit.
-  - exact (fun z => (fst z , (snd z , tt))).
-  - intros z1 z2 p ; cbn.
-    repeat split ; auto.
-    + apply p.
-    + apply p.
-Defined.
-  
-Definition poly_WMalgebra
-           {B : Type} {F : Type}
-           (X : afs B F)
-           (P : forall (f : F), poly ∙ (arity X f))
-           (app : forall (A1 A2 : ty B), poly ((A1 ⟶ A2) ,, A1 ,, ∙) A2)
-           (H1 : forall (A1 A2 : ty B)
-                        (f : weakMonotoneMap
-                               (sem_Ty (fun _ : B => nat_CompatRel) A1)
-                               (sem_Ty (fun _ : B => nat_CompatRel) A2))
-                        (x : sem_Ty (fun _ : B => nat_CompatRel) A1),
-               sem_poly (app A1 A2) (f, (x, tt)) >= f x)
-           (H2 : forall (A1 A2 : ty B)
-                        (f1 f2 : weakMonotoneMap
-                                   (sem_Ty (fun _ : B => nat_CompatRel) A1)
-                                   (sem_Ty (fun _ : B => nat_CompatRel) A2))
-                        (x : sem_Ty (fun _ : B => nat_CompatRel) A1),
-               (forall z, f1 z > f2 z)
-               ->
-               sem_poly (app A1 A2) (f1, (x, tt))
-               >
-               sem_poly (app A1 A2) (f2 , (x , tt)))
-           (H3 : forall (A1 A2 : ty B)
-                        (f : weakMonotoneMap
-                               (sem_Ty (fun _ : B => nat_CompatRel) A1)
-                               (sem_Ty (fun _ : B => nat_CompatRel) A2))
-                        (x1 x2 : sem_Ty (fun _ : B => nat_CompatRel) A1),
-               x1 > x2
-               ->
-               sem_poly (app A1 A2) (f, (x1, tt))
-               >
-               sem_poly (app A1 A2) (f, (x2, tt)))
-           (H4 : forall (r : rewriteRules X)
-                        (x : sem_Con (fun _ : B => nat_CompatRel) (vars r)),
-               sem_Tm
-                 (fun _ : B => nat_CompatRel)
-                 (fun f : F => sem_poly (P f) tt)
-                 (fun A1 A2 : ty B =>
-                    comp_WM
-                      (prod_unit_map
-                         (sem_Ty (fun _ : B => nat_CompatRel) (A1 ⟶ A2))
-                         (sem_Ty (fun _ : B => nat_CompatRel) A1))
-                      (sem_poly (app A1 A2)))
-                 (lhs r)
-                 x
-               >
-               sem_Tm
-                 (fun _ : B => nat_CompatRel)
-                 (fun f : F => sem_poly (P f) tt)
-                 (fun A1 A2 : ty B =>
-                    comp_WM
-                      (prod_unit_map
-                         (sem_Ty (fun _ : B => nat_CompatRel) (A1 ⟶ A2))
-                         (sem_Ty (fun _ : B => nat_CompatRel) A1))
-                      (sem_poly (app A1 A2)))
-                 (rhs r)
-                 x)
-  : WMalgebra X.
-Proof.
-  simple refine (make_WMalgebra
-                   X
-                   (fun _ => nat_CompatRel)
-                   (fun _ => 0)
-                   (fun _ => nat_Wf)
-                   _
-                   (fun f => sem_poly (P f) tt)
-                   (fun A1 A2 => comp_WM (prod_unit_map _ _) (sem_poly (app A1 A2)))
-                   H1 H2 H3 _).
-  - intros r C s x.
-    rewrite !sub_Lemma.
-    apply H4.
-Defined.
- *)
- *)
