Code/Prelude/Orders.v
@@ -1,0 +1,3 @@
+Require Export Prelude.Orders.CompatibleRelation.
+Require Export Prelude.Orders.MonotonicMaps.
+Require Export Prelude.Orders.Examples.
