Code/Prelude/Orders/MonotonicMaps.v
@@ -1,0 +1,136 @@
+Require Import Prelude.Funext.
+Require Import Prelude.Basics.
+Require Import Prelude.Props.
+Require Import Prelude.WellfoundedRelation.
+Require Import Prelude.Orders.CompatibleRelation.
+Require Import Lia.
+Require Import Coq.Program.Equality.
+
+(** * Monotone maps *)
+
+(** We have two kinds of structure preserving maps between compatible relations. First of all, we can look at strictly monotone maps, which preserve the strict order. *)
+Class strictMonotone {X Y : CompatRel} (f : X -> Y) :=
+  map_gt : forall (x y : X),
+    x > y -> f x > f y.
+
+Global Instance strictMonotone_isaprop
+       {X Y : CompatRel}
+       `{isCompatRel Y}
+       (f : X -> Y)
+  : isaprop (strictMonotone f).
+Proof.
+  unfold strictMonotone.
+  apply _.
+Qed.
+
+(** Second of all, we can look at weak monotone maps, which preserve the other order *)
+Class weakMonotone {X Y : CompatRel} (f : X -> Y) :=
+  map_ge : forall (x y : X),
+    x >= y -> f x >= f y.
+
+Global Instance weakMonotone_isaprop
+       {X Y : CompatRel}
+       `{isCompatRel Y}
+       (f : X -> Y)
+  : isaprop (weakMonotone f).
+Proof.
+  unfold weakMonotone.
+  apply _.
+Qed.
+
+(** The weakly monotone maps between two compatible relations forms again a compatible relation *)
+Record weakMonotoneMap (X Y : CompatRel) :=
+  make_monotone
+    {
+      fun_carrier :> X -> Y ;
+      is_weak_monotone : weakMonotone fun_carrier
+    }.
+
+Arguments make_monotone {_ _} _ _.
+
+Global Instance weakMonotoneMap_isWeakMonotone
+       {X Y : CompatRel}
+       (f : weakMonotoneMap X Y)
+  : weakMonotone f
+  := is_weak_monotone _ _ f.
+
+Record strongMonotoneMap (X Y : CompatRel) :=
+  make_strong_monotone
+    {
+      strong_fun_carrier :> X -> Y ;
+      strong_is_weak : weakMonotone strong_fun_carrier ;
+      strong_is_strict : strictMonotone strong_fun_carrier ;
+    }.
+
+Arguments make_strong_monotone {_ _} _ _ _.
+
+Global Instance strongMonotone_to_strictMonotone
+                {X Y : CompatRel}
+                (f : strongMonotoneMap X Y)
+  : strictMonotone f
+  := strong_is_strict _ _ f.
+
+Global Instance strongMonotone_to_weakMonotone
+                {X Y : CompatRel}
+                (f : strongMonotoneMap X Y)
+  : weakMonotone f
+  := strong_is_weak _ _ f.
+
+(** * Equality of monotone maps *)
+Definition eq_weakMonotoneMap_help
+           {X Y : CompatRel}
+           `{isCompatRel Y}
+           (f g : weakMonotoneMap X Y)
+           (p : fun_carrier _ _ f = fun_carrier _ _ g)
+  : f = g.
+Proof.
+  destruct f as [f Hf].
+  destruct g as [g Hg].
+  cbn in p.
+  revert Hf Hg.
+  rewrite p.
+  intros Hf Hg.
+  f_equal.
+  apply all_eq.
+Qed.
+
+Definition eq_weakMonotoneMap
+           {X Y : CompatRel}
+           `{isCompatRel Y}
+           (f g : weakMonotoneMap X Y)
+           (p : forall (x : X), f x = g x)
+  : f = g.
+Proof.
+  apply eq_weakMonotoneMap_help.
+  apply funext.
+  exact p.
+Qed.
+
+Definition eq_strongMonotoneMap_help
+           {X Y : CompatRel}
+           `{isCompatRel Y}
+           (f g : strongMonotoneMap X Y)
+           (p : strong_fun_carrier _ _ f = strong_fun_carrier _ _ g)
+  : f = g.
+Proof.
+  destruct f as [ f Hf1 Hf2 ].
+  destruct g as [ g Hg1 Hg2 ].
+  cbn in p.
+  revert Hf1 Hf2 Hg1 Hg2.
+  rewrite p.
+  intros Hf1 Hf2 Hg1 Hg2.
+  f_equal ; apply all_eq.
+Qed.
+
+Definition eq_strongMonotoneMap
+           {X Y : CompatRel}
+           `{isCompatRel Y}
+           (f g : strongMonotoneMap X Y)
+           (p : forall (x : X), f x = g x)
+  : f = g.
+Proof.
+  apply eq_strongMonotoneMap_help.
+  apply funext.
+  exact p.
+Qed.
+
